Fixed some problems in the random oracle specifiactions

examples/relational/ro.fst
@@ -21,7 +21,12 @@ type tag = b:bytes{length(b)=eta}
 
 (* TODO? *)
 (* an abstract relational predicate on correctly-generated entries *) 
-assume logic type safe (k:key) (t:tag) 
+assume logic type safe_key (k0:key) (k1:key) 
+let safe_key_unique = assume (forall k0 k1 k1'. 
+                               (safe_key k0 k1 /\ safe_key k0 k1' ==> k1 = k1'))
+let safe_key_unique' = assume (forall k0 k0' k1. 
+                               (safe_key k0 k1 /\ safe_key k0' k1 ==> k0 = k0'))
+assume logic type safe (k0:key) (k1:key) (t0:tag) (t1:tag) 
 
 
 type alloc = 
@@ -37,7 +42,7 @@ type state =
 
 type Ok : log -> log -> Type = 
   | Null: Ok [] [] 
-  | ConsH: k0:key -> k1:key-> t0:tag{safe k0 t0} -> t1:tag{safe k1 t1} 
+  | ConsH: k0:key -> k1:key{safe_key k0 k1} -> t0:tag -> t1:tag{safe k0 k1 t0 t1} 
            -> log0:log{is_None (assoc k0 log0)} 
            -> log1:log{is_None (assoc k1 log1)} 
            -> p: Ok log0 log1 
@@ -58,6 +63,8 @@ let rec ok_adv_eq l0 l1 p k = match p with
         | ConsH _ _ _ _ tl0 tl1 p' -> ok_adv_eq tl0 tl1 p' k
         | ConsA _ _ tl0 tl1 p' -> ok_adv_eq tl0 tl1 p' k
 
+assume val ok_witness : l0:log -> l1:log {Ok l0 l1} -> Ok l0 l1
+
 (* Is there any way to show this using the previous lemma? *)
 val ok_adv_eq' : k:key 
                 -> Lemma 
@@ -67,28 +74,42 @@ val ok_adv_eq' : k:key
                                          assoc k l1 = Some(Adv, t))))
 let ok_adv_eq' k = admit ()
 
-
-val ok_hon_safe : l0:log -> l1:log -> p:Ok l0 l1 -> k:key 
-                  -> Lemma 
-                     (requires True)
-                     (ensures (
-                                (forall t. assoc k l0 = Some(Hon, t) ==> safe k t)
-                                /\ (forall t. assoc k l1 = Some(Hon, t) ==> safe k t)))
-let rec ok_hon_safe l0 l1 p k = match p with
-        | Null -> ()
-        | ConsH _ _ _ _ tl0 tl1 p' -> ok_hon_safe tl0 tl1 p' k
-        | ConsA k' t' tl0 tl1 p' -> ok_hon_safe tl0 tl1 p' k
-
-(* Is there any way to show this using the previous lemma? *)
-val ok_hon_safe' : k:key 
+val ok_hon_safe : k0:key -> k1:key -> l0:log -> l1:log -> p:Ok l0 l1
                 -> Lemma 
-                   (requires True)
-                   (ensures (forall (l0:log) (l1:log).Ok l0 l1 ==> 
-                              (forall t. assoc k l0 = Some(Hon, t) ==> safe k t) 
-                              /\ (forall t. assoc k l1 = Some(Hon, t) ==> safe k t)))
-let ok_hon_safe' k = admit ()
+                   (requires (safe_key k0 k1))
+                   (ensures ( (is_Some(assoc k0 l0) /\ is_Hon(fst (Some.v(assoc k0 l0)))) <==>
+                               is_Some(assoc k1 l1) /\ is_Hon(fst (Some.v(assoc k1 l1)))))
+let rec ok_hon_safe k0 k1 l0 l1 p = match p with
+        | Null -> ()
+        | ConsH k0' k1' t01 t1' tl0 tl1 p' -> ok_hon_safe k0 k1 tl0 tl1 p'
+        | ConsA k' t' tl0 tl1 p' -> ok_hon_safe k0 k1 tl0 tl1 p' 
 
-  
+val ok_hon_safe' : k0:key -> k1:key 
+                -> Lemma 
+                   (requires (safe_key k0 k1))
+                   (ensures (forall (l0:log) (l1:log). Ok l0 l1 ==>
+                              (is_Some(assoc k0 l0) /\ is_Hon(fst (Some.v(assoc k0 l0)))) <==>
+                               is_Some(assoc k1 l1) /\ is_Hon(fst (Some.v(assoc k1 l1)))))
+let ok_hon_safe' k0 k1 = admit ()
+
+val ok_hon_safe2 : k0:key -> k1:key -> l0:log -> l1:log -> p:Ok l0 l1
+                -> Lemma 
+                   (requires (safe_key k0 k1))
+                   (ensures (is_Some(assoc k0 l0) /\ is_Hon(fst(Some.v(assoc k0 l0))) ==> 
+                               is_Some(assoc k1 l1) /\ 
+                               safe k0 k1 (snd(Some.v(assoc k0 l0))) (snd(Some.v(assoc k1 l1)))))
+let rec ok_hon_safe2 k0 k1 l0 l1 p = match p with
+        | Null -> ()
+        | ConsH k0' k1' t01 t1' tl0 tl1 p' -> ok_hon_safe2 k0 k1 tl0 tl1 p'
+        | ConsA k' t' tl0 tl1 p' -> ok_hon_safe2 k0 k1 tl0 tl1 p' 
+
+assume val ok_hon_safe'' : k0:key -> k1:key 
+                -> Lemma 
+                   (requires (safe_key k0 k1))
+                   (ensures (forall (l0:log) (l1:log). Ok l0 l1 ==> 
+                                (is_Some(assoc k0 l0) /\ is_Hon(fst(Some.v(assoc k0 l0))) ==> 
+                                  is_Some(assoc k1 l1) /\ 
+                                  safe k0 k1 (snd(Some.v(assoc k0 l0))) (snd(Some.v(assoc k1 l1))))))
 
 type goodstate (s1:state) (s2:state) = 
             s1.bad = true \/ s2.bad = true \/ Ok s1.l s2.l
@@ -97,7 +118,7 @@ assume val s : ref state
 assume val sample_hon : k0:key -> k1:key -> 
                  ST2 (tag * tag)
                    (requires (fun _ -> True))
-                   (ensures (fun h2' p h2 -> h2' = h2 /\ safe k0 (fst p) /\ safe k1 (snd p)))
+                   (ensures (fun h2' p h2 -> h2' = h2 /\ safe k0 k1 (fst p) (snd p)))
 assume val sample_adv : unit -> 
                  ST2 (tag * tag)
                    (requires (fun _ -> True))
@@ -105,11 +126,12 @@ assume val sample_adv : unit ->
 
 val hash_hon:  k0:key -> k1:key ->
                ST2 (option tag * option tag)
-               (requires (fun h2 -> goodstate (sel (fst h2) s) (sel (snd h2) s)))
+               (requires (fun h2 -> goodstate (sel (fst h2) s) (sel (snd h2) s) /\
+                          safe_key k0 k1))
                (ensures (fun _ p h2 -> (sel (fst h2) s).bad \/ 
                                        (sel (snd h2) s).bad \/ 
                                        is_Some (fst p) /\ is_Some (snd p) /\ 
-                                          safe k0 (Some.v(fst p)) /\ safe k1 (Some.v(snd p))))
+                                          safe k0 k1 (Some.v(fst p)) (Some.v(snd p))))
 
 val hash_adv:  k:key -> 
                ST2 (option tag * option tag)
@@ -124,21 +146,23 @@ val add_some : tag -> Tot (option tag)
 let add_some t = Some t
 
 let hash_hon' k r = match assoc k (!s).l with 
-  | Some (Hon,t) -> add_some t 
+  | Some (Hon,t) -> Some t
   | Some (Adv,t) -> s := {bad = true; l = (!s).l}; None
   | None         -> let t = r in 
                     s := {bad = (!s).bad; l= (k,(Hon,t))::(!s).l} ; 
                     add_some t 
 
-let hash_hon k0 k1  = ok_hon_safe' k0;
-                      ok_hon_safe' k1;
+assume val cheat : k0:key -> k1:key -> t0:tag -> t1:tag -> Lemma(safe k0 k1 t0 t1)
+
+let hash_hon k0 k1  = ok_hon_safe' k0 k1;
+                      ok_hon_safe'' k0 k1;
                       let r0, r1 = sample_hon k0 k1 in 
                       (compose2 (fun k -> hash_hon' k r0) 
                                 (fun k -> hash_hon' k r1) 
                                 k0 k1)
 
 let hash_adv' k r =  match assoc k (!s).l with 
-  | Some (Adv,t) -> add_some t 
+  | Some (Adv,t) -> Some t 
   | Some (Hon,t) -> s := {bad = true; l = (!s).l}; None
   | None         -> let t = r in 
                     s := {bad = (!s).bad; l= (k,(Adv,t))::(!s).l} ; 
